Fix constant propagation.

theories/ValueOpts/ConstantPropagationAnalysis.v
@@ -10,7 +10,6 @@ Set Implicit Arguments.
 
 Open Scope map_scope.
 
-
 Definition Dom := Map [var, withTop val].
 
 
@@ -29,23 +28,41 @@ Smpl Add 100 match goal with
 
 Require Import MapNotations ListUpdateAt Subterm.
 
+Lemma WithTopLe_refl A R `{EqDec A R} (a b : A)
+  : R a b
+    -> poLe (wTA a) (wTA b).
+Proof.
+  econstructor; eauto.
+Qed.
+
+Lemma poLe_Some_struct A `{PartialOrder A} (a b : A)
+  : poLe a b
+    -> poLe (Some a) (Some b).
+Proof.
+  econstructor; eauto.
+Qed.
+
+Lemma poLe_withTopLe_top A R `{EqDec A R} (x:withTop A)
+  : poLe x Top.
+Proof.
+  econstructor 2.
+Qed.
+
+
 Lemma leMap_op_eval e a b
   : poLe a b
     -> poLe (op_eval (domenv a) e) (op_eval (domenv b) e).
 Proof.
-  general induction e; simpl; eauto using @fstNoneOrR, @withTop_le.
-  - reflexivity.
-  - unfold domenv.
-    specialize (H n).
-    destruct (find n a); eauto using fstNoneOrR.
-  - specialize (IHe _ _ H); repeat cases; eauto using fstNoneOrR, @withTop_le.
-    reflexivity.
+  revert a b.
+  general induction e; simpl; eauto.
+  - specialize (IHe _ _ H).
+    repeat cases; clear_trivial_eqs;
+      eauto using poLe_option_None, poLe_withTopLe_top, poLe_Some_struct.
   - specialize (IHe1 _ _ H).
     specialize (IHe2 _ _ H).
     inv IHe1; inv IHe2; repeat cases;
       simpl in *; clear_trivial_eqs;
-        eauto using fstNoneOrR, withTop_le.
-    + econstructor; econstructor. congruence.
+        eauto using poLe_option_None, poLe_withTopLe_top, poLe_Some_struct.
 Qed.
 
 Hint Resolve leMap_op_eval.
@@ -54,23 +71,19 @@ Lemma eqMap_op_eval e a b
   : poEq a b
     -> poEq (op_eval (domenv a) e) (op_eval (domenv b) e).
 Proof.
-  general induction e; simpl; eauto using @fstNoneOrR, @withTop_eq, @option_R.
-  - reflexivity.
-  - unfold domenv.
-    specialize (H n).
-    destruct (find n a); eauto using fstNoneOrR.
-  - specialize (IHe _ _ H); repeat cases; eauto using fstNoneOrR, @withTop_eq, @option_R.
-    reflexivity.
+  revert a b.
+  general induction e; simpl; eauto.
+  - specialize (IHe _ _ H).
+    repeat cases; clear_trivial_eqs;
+      eauto using poLe_option_None, poLe_withTopLe_top, poLe_Some_struct.
   - specialize (IHe1 _ _ H).
     specialize (IHe2 _ _ H).
     inv IHe1; inv IHe2; repeat cases;
       simpl in *; clear_trivial_eqs;
-        eauto using fstNoneOrR, withTop_eq, option_R.
-    + econstructor; econstructor. congruence.
+        eauto using poLe_option_None, poLe_withTopLe_top, poLe_Some_struct.
 Qed.
 
 Hint Resolve leMap_op_eval eqMap_op_eval.
-
 
 Definition DDom (sT:stmt) := { m : Map [var, withTop val] | domain m ⊆ occurVars sT}.
 
@@ -78,44 +91,6 @@ Smpl Add match goal with
          | [ H : poLe _ None |- _ ] => invc H
          | [ H : ⎣ ?x ⎦ <> ⎣ ?x ⎦ |- _ ] => exfalso; apply H; reflexivity
          end : inv_trivial.
-
-Lemma cp_trans_reach_mon
-  : forall (sT : stmt) (e : op) (s : stmt),
-    subTerm s sT ->
-    forall (FVIncl : Op.freeVars e [<=] occurVars sT) (a a' : DDom sT),
-      a ⊑ a' ->
-      forall b b' : bool,
-        b ⊑ b' -> cp_trans_reach e FVIncl a b ⊑ cp_trans_reach e FVIncl a' b'.
-Proof.
-  intros. pose proof (leMap_op_eval e H0); eauto.
-  unfold cp_trans_reach.
-  set (X:=op_eval (domenv (proj1_sig a)) e) in *.
-  set (Y:=op_eval (domenv (proj1_sig a')) e) in *. clearbody X Y.
-  unfold val in *.
-  repeat cases; split; simpl fst; simpl snd; eauto; clear_trivial_eqs.
-  inv H2; clear_trivial_eqs.
-  inv H2; clear_trivial_eqs.
-Qed.
-
-Lemma cp_trans_reach_ext
-  : forall sT (e : op) (s : stmt),
-    subTerm s sT ->
-    forall (FVIncl : Op.freeVars e [<=] occurVars sT) (a0 a' : DDom sT),
-      a0 ≣ a' ->
-      forall b b' : bool,
-        b ≣ b' -> cp_trans_reach e FVIncl a0 b ≣ cp_trans_reach e FVIncl a' b'.
-Proof.
-  intros. exploit (eqMap_op_eval e); eauto. eapply H0.
-  unfold cp_trans_reach.
-  set (X:=op_eval (domenv (proj1_sig a0)) e) in *.
-  set (Y:=op_eval (domenv (proj1_sig a')) e) in *. clearbody X Y.
-  repeat cases; split; simpl fst; simpl snd; eauto; clear_trivial_eqs;
-  inv H2; clear_trivial_eqs; exfalso; eauto.
-Qed.
-
-
-Definition cp_reach (U : ⦃nat⦄) (b:bool) (d: VDom U (withTop val)) (e:op) : bool * bool :=
-  (true, true).
 
 Definition cp_reach (U : ⦃nat⦄) (b:bool) (d: VDom U (withTop val)) (e:op) : bool * bool :=
   (if [op_eval (domenv (proj1_sig d)) e = None] then false
@@ -128,7 +103,27 @@ Definition cp_reach (U : ⦃nat⦄) (b:bool) (d: VDom U (withTop val)) (e:op) : 
 Lemma cp_reach_mon (U : ⦃nat⦄) (e : op) (a a' : VDom U (withTop val))
   : a ⊑ a' -> forall b b' : bool, b ⊑ b' -> cp_reach b a e ⊑ cp_reach b' a' e.
 Proof.
-  intros. reflexivity.
+  unfold cp_reach.
+  intros.
+  intros. pose proof (leMap_op_eval e H); eauto.
+  set (X:=op_eval (domenv (proj1_sig a)) e) in *.
+  set (Y:=op_eval (domenv (proj1_sig a')) e) in *. clearbody X Y.
+  unfold val in *.
+  repeat cases; split; simpl fst; simpl snd; eauto; clear_trivial_eqs.
+  inv H1; clear_trivial_eqs.
+  inv H1; clear_trivial_eqs.
+Qed.
+
+Lemma cp_reach_ext (U : ⦃nat⦄) (e : op) (a a' : VDom U (withTop val))
+  : a ≣ a' -> forall b b' : bool, b ≣ b' -> cp_reach b a e ≣ cp_reach b' a' e.
+Proof.
+  unfold cp_reach.
+  intros.
+  intros. pose proof (eqMap_op_eval e H); eauto.
+  set (X:=op_eval (domenv (proj1_sig a)) e) in *.
+  set (Y:=op_eval (domenv (proj1_sig a')) e) in *. clearbody X Y.
+  unfold val in *.
+  repeat cases; split; simpl fst; simpl snd; eauto; clear_trivial_eqs.
 Qed.
 
 Definition cp_trans (U : ⦃nat⦄) (b:bool) (d: VDom U (withTop val)) (e:exp) : ؟ (withTop val) :=
@@ -142,6 +137,28 @@ Lemma cp_trans_mon (U : ⦃nat⦄) (e : exp) (a a' : VDom U (withTop val))
 Proof.
   intros. destruct e; simpl; eauto.
 Qed.
+
+Lemma cp_trans_ext (U : ⦃nat⦄) (e : exp) (a a' : VDom U (withTop val))
+  : a ≣ a' -> forall b b' : bool, b ≣ b' -> @cp_trans U b a e ≣ @cp_trans U b' a' e.
+Proof.
+  intros. destruct e; simpl; eauto.
+Qed.
+
+Instance withTop_OUB A R `{EqDec A R}
+  : @UpperBounded (option (withTop A)) _ :=
+  { top := Some Top
+  }.
+- intros.
+  destruct a; eauto using poLe_Some_struct, poLe_withTopLe_top.
+Defined.
+
+Instance withTop_UB A R `{EqDec A R}
+  : @UpperBounded (withTop A) _ :=
+  { top := Top
+  }.
+- intros.
+  eauto using poLe_Some_struct, poLe_withTopLe_top.
+Defined.
 
 Definition constant_propagation_analysis :=
   makeForwardAnalysis _ _ _ cp_trans cp_reach cp_trans_mon cp_reach_mon.
