theories/ValueOpts/ConstantPropagationAnalysisCorrect.v
@@ -5,342 +5,230 @@ Require Import Analysis AnalysisForwardSSA Subterm CSet MapAgreement RenamedApar
 Require Import Infra.PartialOrder Infra.Lattice Infra.WithTop.
 Require Import LabelsDefined Annotation.
 Require Import Reachability ReachabilityAnalysisCorrectSSA.
-Require Import ConstantPropagation ConstantPropagationAnalysis.
+Require Import ConstantPropagation ConstantPropagationAnalysis DomainSSA.
 
 Local Arguments proj1_sig {A} {P} e.
 Local Arguments length {A} e.
-Local Arguments forward {sT} {Dom} ftransform reach_transf ZL ZLIncl st.
-
+Local Arguments forward {sT} {D} {H} {H0} exp_transf reach_transf ZL ZLIncl st ST d anr.
 
 Notation "'getAE' X" := (proj1_sig (fst (fst X))) (at level 10, X at level 0).
 
 Local Arguments exist {A} {P} x _.
-Local Arguments forward {sT} {Dom} ftransform reach_transf ZL {ZLIncl} st {ST}.
-Local Arguments cp_trans_dep {sT} ZL st {ST} {ZLIncl}.
-Local Arguments cp_trans_domain {sT} ZL st {ST} {ZLIncl} a b.
+
+Lemma domenv_map_proper D `{PartialOrder D} Z
+  : Proper (poEq ==> poEq) (fun AE => domenv AE ⊝ Z).
+Proof.
+  unfold Proper, respectful; intros.
+  general induction Z; simpl; eauto using poEq_list_struct.
+Qed.
 
 
+Lemma domjoin_list_domenv D `{JoinSemiLattice D} Z (Y:list (option D)) AE
+  (ND : NoDupA eq Z)
+  (LEN : ❬Z❭ = ❬Y❭)
+  : Y ⊑ domenv (domjoin_list AE Z Y) ⊝ Z.
+Proof.
+  general induction LEN; simpl; eauto.
+  eapply poLe_list_struct.
+  - unfold domenv at 1.
+    rewrite domupd_var_eq; eauto.
+  - eapply PIR2_get; eauto with len.
+    intros; inv_get.
+    unfold domenv. rewrite domupd_var_ne; eauto.
+    exploit IHLEN; eauto.
+    + eapply PIR2_nth in H3; eauto; dcr; inv_get.
+      eapply H6.
+    + intro EQ; invc EQ. inv ND. eapply H5.
+      eapply get_InA in H2. eauto.
+Qed.
 
-Definition cp_sound sT AE AE' AV ZL s (ST:subTerm s sT) ZLIncl ra anr
-  : let X := @forward sT _ (@cp_trans_dep) (@cp_trans_reach) ZL ZLIncl s ST AE anr in
+Definition cp_sound sT AE ZL s (ST:subTerm s sT) ZLIncl ra anr
+  : let X := @forward sT _ _ _ (@cp_trans) (@cp_reach) ZL ZLIncl s ST AE anr in
     renamedApart s ra
     -> annotation s anr
     -> labelsDefined s (length ZL)
     -> poEq (fst X) (AE,anr)
-    -> poEq AE' AE
     -> disj (list_union (of_list ⊝ ZL)) (snd (getAnn ra))
-    -> ❬ZL❭ = ❬AV❭
     -> paramsMatch s (length ⊝ ZL)
-    -> PIR2 eq AV (List.map (fun Z => lookup_list (domenv (proj1_sig AE')) Z) ZL)
     -> (forall n Z, get ZL n Z -> NoDupA eq Z)
-    -> cp_sound (domenv (proj1_sig AE')) (zip pair ZL AV) s anr.
+    -> cp_sound (domenv (proj1_sig AE))
+               (zip pair ZL (lookup_list (domenv (proj1_sig AE)) ⊝ ZL)) s anr.
 Proof.
-  intros LET RA ANN LD EQ1 EQ2 DISJ LEN PM AVREL NODUP. subst LET.
+  intros LET RA ANN LD EQ1 DISJ PM NODUP. subst LET.
   general induction LD; invt @renamedApart;
     try invt @annotation; simpl in *; simpl; invt @paramsMatch;
       simpl in *; dcr;
         repeat let_pair_case_eq; repeat let_case_eq; repeat simpl_pair_eqs; subst;
           simpl in *; try invtc @ann_R; subst.
-  - destruct e; simpl in *; simpl in *; clear_trivial_eqs.
-    + assert (EVALEQ:op_eval (domenv (proj1_sig AE')) e = domenv (proj1_sig AE) x). {
-        set_simpl.
-        exploit cp_forward_agree_def as AGR. eauto.
-        eapply setTopAnn_annotation; eauto.
-        instantiate (3:=(domupd (proj1_sig AE) x (op_eval (domenv (proj1_sig AE)) e)))
-          in AGR.
-        instantiate (2:=(cp_trans_domain ZL (stmtLet x (Operation e) s) AE a)) in AGR.
-        exploit (AGR x). pe_rewrite. instantiate (2:={x; Ds}).
-        eapply renamedApart_disj in H4. pe_rewrite.
-        revert H4 DISJ; clear_all. cset_tac.
-        exploit (H x).
-        eapply option_R_inv in H0.
-        eapply option_R_inv in H1. unfold domenv in H0.
-        unfold domenv. rewrite <- H1.
-        unfold domenv.
-        rewrite <- H0.
-        rewrite domupd_eq; eauto.
-        exploit  eqMap_op_eval. eapply EQ2.
-        eapply option_R_inv in H5. eauto.
-      }
-      assert (MAPEQ:eqMap (proj1_sig AE')
-                          (domupd (proj1_sig AE) x (op_eval (domenv (proj1_sig AE)) e))). {
-        rewrite EQ2.
-        eapply eqMap_domupd.
-        unfold domenv in EVALEQ.
-        rewrite <- EVALEQ.
-        rewrite <- eqMap_op_eval; [|eapply EQ2].
-        reflexivity.
-      }
-      simpl_forward_setTopAnn. subst. repeat rewrite setTopAnn_eta' in *.
-      econstructor; eauto.
-      eapply IHLD with (AE:=(exist (domupd (proj1_sig AE) x (op_eval (domenv (proj1_sig AE)) e))
-                      (cp_trans_domain ZL (stmtLet x (Operation e) s) AE (getAnn sa)))); eauto.
-      * split; eauto.
-        -- simpl.
-           etransitivity; eauto.
-           etransitivity; eauto.
-           symmetry; eauto.
-      * pe_rewrite. set_simpl.
-        eapply disj_incl; eauto with cset.
-      * intros; simpl; eauto.
-        rewrite EVALEQ.
-        exploit (EQ2 x). eapply option_R_inv in H1.
-        unfold domenv. congruence.
-    + assert (find x (proj1_sig AE') = ⎣ Top ⎦). {
-        set_simpl.
-        exploit cp_forward_agree_def as AGR. eauto.
-        eapply setTopAnn_annotation; eauto.
-        instantiate (3:=add x Top (proj1_sig AE)) in AGR.
-        instantiate (2:=cp_trans_domain ZL (stmtLet x (Call f Y) s) AE a) in AGR.
-        exploit (AGR x). pe_rewrite. instantiate (2:={x; Ds}).
-        eapply renamedApart_disj in H4. pe_rewrite.
-        revert H4 DISJ; clear_all. cset_tac.
-        exploit (H x).
-        eapply option_R_inv in H0.
-        eapply option_R_inv in H1. unfold domenv in H0.
-        exploit (EQ2 x).
-        eapply option_R_inv in H5. rewrite H5.
-        rewrite <- H1. rewrite <- H0.
-        mlud; eauto. exfalso; eauto.
-      }
-      assert (eqMap (proj1_sig AE') (add x Top (proj1_sig AE))). {
-        hnf; intros. mlud; eauto. rewrite <- e.
-        rewrite <- H0. reflexivity.
-      }
-      simpl_forward_setTopAnn. subst. repeat rewrite setTopAnn_eta' in *.
-      econstructor; eauto.
-      eapply IHLD with (AE:=(exist (add x Top (proj1_sig AE))
-                     (cp_trans_domain ZL (stmtLet x (Call f Y) s) AE (getAnn sa)))); eauto.
-      * split; eauto; simpl.
-        etransitivity; eauto.
-        etransitivity; eauto.
-        symmetry; eauto.
-      * pe_rewrite. set_simpl.
-        eapply disj_incl; eauto with cset.
-  - assert (MEQ: eqMap (proj1_sig AE')
-    (getAE (@forward sT DDom (@cp_trans_dep) (@cp_trans_reach) ZL ZLIncl s (subTerm_EQ_If1 eq_refl ST)
-              (exist (proj1_sig AE) (@cp_trans_domain sT ZL (stmtIf e s t) ST ZLIncl AE a))
-              (setTopAnn sa
-                 (if [op_eval (domenv (proj1_sig AE)) e = ⎣⎦] then false else if [
-                  op_eval (domenv (proj1_sig AE)) e = ⎣ wTA val_false ⎦] then false else a))))). {
-        hnf; intros.
-        edestruct (@cp_forward_agree sT ZL (fst
-                     (fst
-                        (@forward sT DDom (@cp_trans_dep) (@cp_trans_reach) ZL ZLIncl s
-                                  (subTerm_EQ_If1 eq_refl ST)
-                           (exist (proj1_sig AE)
-                              (@cp_trans_domain sT ZL (stmtIf e s t) ST ZLIncl AE a))
-                           (setTopAnn sa
-                              (if [op_eval (domenv (proj1_sig AE)) e = ⎣⎦] then false else if [
-                               op_eval (domenv (proj1_sig AE)) e =
-                               ⎣ wTA val_false ⎦] then false else a)))))). eauto.
-        eapply setTopAnn_annotation; eauto.
-        instantiate (4:=singleton x) in H1. pe_rewrite.
-        decide (x ∈ (Dt ∪ list_union (of_list ⊝ ZL))).
-        -- edestruct (@cp_forward_agree sT ZL (exist (proj1_sig AE) (@cp_trans_domain sT ZL (stmtIf e s t) ST ZLIncl AE a)) (singleton x) s). eauto.
-           eapply setTopAnn_annotation; eauto.
-           pe_rewrite.
-           assert ((x ∈ Dt /\ x ∉ list_union (of_list ⊝ ZL))
-                   \/ (x ∈ list_union (of_list ⊝ ZL) /\ x ∉ Dt /\ x ∉ Ds)). {
-             revert i DISJ H4.
-             clear_all; cset_tac.
-           } destruct H15; dcr.
-           ++ exploit (H7 x).
-             revert H17 H18 H3 i; clear_all. cset_tac.
-             unfold domenv in H15.
-             etransitivity; eauto.
-           ++ etransitivity; eauto.
-             eapply poLe_antisymmetric.
-             eapply H14. revert H22; clear_all; cset_tac.
-             etransitivity.
-             eapply H1. revert H21; clear_all; cset_tac.
-             exploit (H x).
-             rewrite <- H15. unfold domenv. reflexivity.
-        -- exploit (H0 x). revert n; clear_all. cset_tac.
-           rewrite H7.
-           etransitivity. eapply EQ2.
-           symmetry. exploit (H x).
-           rewrite <- H14.
-           unfold domenv. reflexivity.
-    }
-    simpl_forward_setTopAnn. subst. repeat rewrite setTopAnn_eta' in *.
-    symmetry in HEQ. symmetry in HEQ0.
-    rewrite <- (setTopAnn_eta _ HEQ0).
-    rewrite <- (setTopAnn_eta _ HEQ).
-    econstructor; eauto.
-    + eapply IHLD1.
-      * eauto.
-      * eauto using setTopAnn_annotation.
-      * eauto.
-      * split.
-        -- etransitivity.
-           symmetry.
-           eapply MEQ. simpl. eauto.
-        -- eapply ann_R_setTopAnn_right; eauto.
-           ++ rewrite forward_fst_snd_getAnn.
-             rewrite getAnn_setTopAnn; eauto.
-      * simpl. eauto.
-      * pe_rewrite. clear MEQ. set_simpl.
-        eapply disj_incl. eapply DISJ.
-        eauto. eauto with cset.
-      * eauto.
-      * eauto.
-      * eauto.
-      * eauto.
-    + eapply IHLD2; eauto.
-      * eapply setTopAnn_annotation. eauto.
-      * split.
-        -- etransitivity; eauto.
-           etransitivity; eauto.
-           symmetry; eauto.
-        -- etransitivity; eauto.
-           eapply ann_R_setTopAnn_right; eauto.
-      * clear MEQ.
-        pe_rewrite. set_simpl.
-        eapply disj_incl. eapply DISJ.
-        reflexivity. eauto with cset.
-  - econstructor.
-  - clear_trivial_eqs. set_simpl.
-    edestruct get_in_range; eauto.
-    erewrite get_nth in *; eauto.
-    inv_get.
-    edestruct PIR2_nth; eauto using map_get_1, ListUpdateAt.list_update_at_get_3; dcr.
-    econstructor; eauto using zip_get; intros.
-    + PIR2_inv; clear_trivial_eqs; inv_get.
-      eapply PIR2_get.
-      * rewrite lookup_list_map.
-        intros; inv_get.
-        exploit (H0 x1) as EQA. unfold domenv.
-        exploit (EQ2 x1) as EQB. rewrite <- EQA in EQB.
-        rewrite EQB.
-        cases.
-        exploit domupd_list_get; [|eapply H6| eapply map_get_1; try eapply H5|].
-        -- exploit NODUP; eauto.
-        -- etransitivity;[| eapply H7].
-           exploit eqMap_op_eval; try eapply EQ2.
-           eapply option_R_inv in H8.
-           unfold domenv in H8.
-           rewrite H8. reflexivity.
-      * rewrite map_length. rewrite lookup_list_length; eauto.
-  -
-    assert (ZipEq:((fun Zs0 : params * stmt => (fst Zs0, lookup_list (domenv (proj1_sig AE')) (fst Zs0))) ⊝ F ++ pair ⊜ ZL AV) = (zip pair (fst ⊝ F ++ ZL) ((fun Zs => lookup_list (domenv (proj1_sig AE')) (fst Zs)) ⊝ F ++ AV))). {
-      clear_all. general induction F; simpl; eauto.
-      f_equal. eapply IHF.
-    }
-    simpl_forward_setTopAnn. subst. repeat rewrite setTopAnn_eta' in *.
-    assert (joinTopAnn (A:=bool) ⊜ sa (snd (@forward _ _ (@cp_trans_dep) (@cp_trans_reach) (fst ⊝ F ++ ZL) (ZLIncl_ext ZL eq_refl ST ZLIncl) t (subTerm_EQ_Fun1 eq_refl ST) AE ta)) = sa). {
-      eapply PIR2_eq.
-      eapply PIR2_R_impl. intros.
-      eapply ann_R_eq. eapply H2.
-      eapply snd_forwarF_inv; eauto.
-      clear. eauto with len.
-      rewrite forward_length. reflexivity.
-      eapply PIR2_get in H23; eauto.
-    }
-    exploit eqMap_forwardF_t; eauto.
-    clear. len_simpl. omega.
-    reflexivity. pe_rewrite. set_simpl.
-    eapply funConstr_disj_Dt'; eauto.
-    pe_rewrite.
-    rewrite list_union_defVars_decomp in *; eauto. set_simpl.
-    eapply disj_Dt_getAnn; eauto.
-    set_simpl.
-    eapply funConstr_disj_ZL_getAnn; eauto.
-    set_simpl.
-    eapply disj_1_incl.
-    eapply funConstr_disj_ZL_getAnn; eauto.
-    rewrite List.map_app. rewrite list_union_app.
-    clear_all. cset_tac.
-    revert H9. clear_all. len_simpl. intros. rewrite H9. eauto with len.
-    intros. inv_get. eapply setTopAnn_annotation. eauto.
-    econstructor; eauto.
-    + intros; inv_get.
-      setoid_rewrite ZipEq.
-      pose proof H16 as GET.
-      assert (FWDP:forall STZs, PIR2 impb (snd (@forward _ _ (@cp_trans_dep) (@cp_trans_reach) (fst ⊝ F ++ ZL) (ZLIncl_ext ZL eq_refl ST ZLIncl) (snd Zs) STZs AE r))
-                                (snd
-                                   (forwardF (snd (@forward _ _ (@cp_trans_dep) (@cp_trans_reach) (fst ⊝ F ++ ZL) (ZLIncl_ext ZL eq_refl ST ZLIncl) t ((subTerm_EQ_Fun1 eq_refl ST)) AE ta))
-                                             (@forward _ _ (@cp_trans_dep) (@cp_trans_reach) (fst ⊝ F ++ ZL) (ZLIncl_ext ZL eq_refl ST ZLIncl)) F
-                                             (joinTopAnn (A:=bool) ⊜ sa
-                                                         (snd (@forward _ _ (@cp_trans_dep) (@cp_trans_reach) (fst ⊝ F ++ ZL) (ZLIncl_ext ZL eq_refl ST ZLIncl) t ((subTerm_EQ_Fun1 eq_refl ST)) AE ta)))
-                                             AE
-                                             (subTerm_EQ_Fun2 eq_refl ST)))). {
+  - set_simpl. clear_trivial_eqs.
+    + pose proof EQ1 as EQ3.
+      eapply forward_domupdd_eq in EQ3; eauto.
+      * econstructor; eauto.
+        eapply IHLD; eauto.
+        split; simpl. rewrite <- EQ1 at 2.
+        eapply forward_ext; eauto using cp_trans_ext, cp_reach_ext.
+        rewrite <- EQ3. symmetry; eauto.
+        rewrite <- H10 at 2.
+        eapply forward_ext; eauto using cp_trans_ext, cp_reach_ext.
+        rewrite <- EQ3. symmetry; eauto.
+        pe_rewrite. eauto with cset.
         intros.
-        eapply forwardF_PIR2.
-        +++ revert H9. clear_all; intros; len_simpl.
-           rewrite H9. eauto with len.
-        +++ clear_all. eauto with len.
-        +++ intros.
-           inv_get.
-           destruct H14.
-           eapply H26; eauto.
-           eapply zip_get; eauto.
-        +++ eapply transf_ext.
-        +++ eapply cp_trans_reach_ext.
-        +++ rewrite H2. eauto.
-        +++ eauto.
+        rewrite EQ1 in EQ3.
+        specialize (EQ3 x). unfold domenv.
+        eapply option_R_inv in EQ3.
+        rewrite EQ3. simpl. rewrite domupd_var_eq; try reflexivity.
+      * rewrite renamedApart_occurVars; eauto. pe_rewrite.
+        eapply renamedApart_disj in H4; eauto.
+        pe_rewrite. revert DISJ H4; clear_all; cset_tac.
+  - clear_trivial_eqs.
+    set_simpl.
+    exploit (forward_if_inv _ _ _ _ _ _ EQ1); eauto.
+    repeat rewrite renamedApart_occurVars; eauto;
+      pe_rewrite; eauto with cset.
+    repeat rewrite renamedApart_occurVars; eauto;
+      pe_rewrite; eauto with cset.
+    rewrite forward_ext in EQ1; eauto using cp_reach_ext, cp_trans_ext; try reflexivity.
+    econstructor; eauto.
+    + eapply IHLD1; eauto.
+      split; eauto. pe_rewrite. eauto with cset.
+    + eapply IHLD2; eauto.
+      split; eauto.
+      rewrite forward_ext; eauto using cp_reach_ext, cp_trans_ext. symmetry; eauto.
+      pe_rewrite. eapply disj_2_incl; eauto with cset.
+  - econstructor; eauto.
+  - inv_get.
+    econstructor; eauto using zip_get_eq.
+    intros. cases in EQ1. inv_get.
+    set_simpl.
+    unfold domjoin_listd in EQ1.
+    destruct AE as [AE pf]; simpl in *; clear_trivial_eqs.
+    unfold poEq in EQ1. simpl in EQ1.
+    rewrite (get_nth nil H3) in *.
+    exploit NODUP; eauto.
+    rewrite lookup_list_map.
+    symmetry in EQ1.
+    rewrite domenv_map_proper; eauto.
+    eapply domjoin_list_domenv; eauto with len.
+  - clear_trivial_eqs.
+    eapply PIR2_get in H21; try eassumption. clear H20.
+    exploit (snd_forwardF_inv _ _ _ _ _ _ _ H21); eauto with len.
+    exploit (snd_forwardF_inv' _ _ _ _ _ _ _ H21); eauto with len.
+    Transparent poEq. simpl poEq in H21.
+    repeat PIR2_eq_simpl. repeat ST_pat.
+    Opaque poEq.
+    set (FWt:=(forward cp_trans cp_reach (fst ⊝ F ++ ZL) ZLIncl0 t ST0 AE ta)) in *.
+    set (FWF:=forwardF (snd FWt) (forward cp_trans cp_reach (fst ⊝ F ++ ZL) ZLIncl0)
+                       F sa (fst (fst FWt)) STF) in *.
+    assert (fst (fst (FWt)) ≣ AE /\
+            forall (n : nat) (Zs : params * stmt) (r : ann bool) (ST0 : subTerm (snd Zs) sT),
+              get F n Zs ->
+              get sa n r ->
+              fst
+                (fst
+                   (forward cp_trans cp_reach (fst ⊝ F ++ ZL) (ZLIncl_ext ZL eq_refl ST ZLIncl) (snd Zs) ST0 AE r))
+                ≣ AE). {
+      pe_rewrite. set_simpl.
+      eapply forwardF_agree_get; eauto. eauto with len.
+      rewrite <- EQ1. unfold FWF. reflexivity.
+      unfold FWt. reflexivity.
+      pe_rewrite. eauto with ren.
+      pe_rewrite.
+      eapply disj_Dt_getAnn; eauto.
+      eapply funConstr_disj_ZL_getAnn; eauto.
+      eapply disj_1_incl.
+      eapply funConstr_disj_ZL_getAnn; eauto.
+      rewrite List.map_app. rewrite list_union_app.
+      clear_all. cset_tac.
+      eapply cp_trans_ext. eapply cp_reach_ext.
+    } dcr.
+
+    assert (forall (n : nat) (r : ann bool) (Zs : params * stmt),
+       get sa n r ->
+       get F n Zs ->
+       forall STZs : subTerm (snd Zs) sT,
+         (snd
+            (fst
+               (forward cp_trans cp_reach (fst ⊝ F ++ ZL)
+                        ZLIncl0 (snd Zs) STZs AE r))) ≣ r). {
+      eapply (@snd_forwardF_inv_get) with (BL:=(snd FWt)); eauto.
+      subst FWt; eauto with len.
+      subst FWt; eauto with len.
+      rewrite <- H2 at 2. unfold FWF.
+      rewrite forwardF_ext'; try reflexivity; eauto.
+      eapply cp_trans_ext; eauto.
+      eapply cp_reach_ext; eauto.
+      symmetry; eauto.
+      eapply cp_trans_ext; eauto.
+      eapply cp_reach_ext; eauto.
+    }
+    econstructor; eauto.
+    + intros. inv_get. exploit H7; eauto.
+      assert (EQ:
+                ((fun Zs0 : params * stmt =>
+      (fst Zs0, lookup_list (domenv (proj1_sig AE)) (fst Zs0))) ⊝ F ++
+     pair ⊜ ZL (lookup_list (domenv (proj1_sig AE)) ⊝ ZL))
+              = zip pair (fst ⊝ F ++ ZL) (lookup_list (domenv (proj1_sig AE)) ⊝ (fst ⊝ F ++ ZL))). {
+        rewrite !List.map_app. rewrite !zip_app; eauto with len.
+        rewrite !zip_map_l. rewrite !zip_map_r.
+        f_equal; eauto.
+        clear_all. general induction F; simpl; f_equal; eauto.
       }
-      eapply H0;
-        eauto.
-      * clear_all; eauto with len.
-      * split.
-        -- eapply H14; eauto.
-           rewrite H2; eauto.
-        -- eapply PIR2_get in H23; eauto.
-           exploit snd_forwarF_inv; eauto.
-           clear; eauto with len.
-           clear; eauto with len.
-           exploit snd_forwarF_inv'; eauto.
-           clear; eauto with len.
-           clear; eauto with len.
-           destruct H14.
-           rewrite (@forwardF_ext sT DDom _
-                                  (@forward _ _ (@cp_trans_dep) (@cp_trans_reach) (fst ⊝ F ++ ZL) (@ZLIncl_ext sT (stmtFun F t) F t ZL (@eq_refl stmt (stmtFun F t)) ST
-                                                                                            ZLIncl)) (@forward _ _ (@cp_trans_dep) (@cp_trans_reach) (fst ⊝ F ++ ZL) (@ZLIncl_ext sT (stmtFun F t) F t ZL (@eq_refl stmt (stmtFun F t)) ST
-                   ZLIncl))) in H20;
-             try eapply e; intros; try reflexivity.
-           eapply snd_forwarF_inv_get; try eapply H20; eauto.
-           clear; eauto with len.
-           clear; eauto with len.
-           intros.
-           eapply PIR2_nth_2 in H19; eauto; dcr.
-           intros. eapply p; eauto.
-           rewrite ann_R_eq in H27. subst. eauto.
-           eapply forward_ext; eauto.
-           eapply transf_ext; eauto.
-           eapply cp_trans_reach_ext; eauto.
-      * set_simpl. eauto.
-        eapply disj_2_incl.
-        eapply funConstr_disj_ZL_getAnn; eauto.
-        eapply incl_list_union; eauto using zip_get.
-      * revert LEN; clear_all; eauto with len.
-      * rewrite List.map_app.
-        eapply PIR2_app; eauto.
-        eapply PIR2_get; intros; inv_get. reflexivity.
-        clear_all.
-        eauto with len.
-      * intros ? ? GET2. eapply get_app_cases in GET2. destruct GET2.
-        inv_get. edestruct H5; eauto.
-        dcr. inv_get. eapply NODUP; eauto.
-    + setoid_rewrite ZipEq.
-      eapply IHLD; eauto.
-      * clear; eauto with len.
-      * split; dcr. eauto. eauto.
+      rewrite EQ.
+      eapply H0; eauto.
+      -- eauto with len.
+      -- split; simpl; eauto.
+      -- set_simpl.
+         eapply disj_2_incl.
+         eapply funConstr_disj_ZL_getAnn; eauto with ren.
+         eapply incl_list_union; eauto using zip_get.
+      -- intros ? ? GET2. eapply get_app_cases in GET2. destruct GET2.
+         inv_get. edestruct H5; eauto.
+         dcr. inv_get. eapply NODUP; eauto.
+    + assert (EQ:
+                (fun Zs : params * stmt => (fst Zs, lookup_list (domenv (proj1_sig AE)) (fst Zs)))
+                  ⊝ F ++ pair ⊜ ZL (lookup_list (domenv (proj1_sig AE)) ⊝ ZL)
+                = zip pair (fst ⊝ F ++ ZL) (lookup_list (domenv (proj1_sig AE)) ⊝ (fst ⊝ F ++ ZL))). {
+        rewrite !List.map_app. rewrite !zip_app; eauto with len.
+        rewrite !zip_map_l. rewrite !zip_map_r.
+        f_equal; eauto.
+        clear_all. general induction F; simpl; f_equal; eauto.
+      }
+      rewrite EQ.
+      eapply IHLD; eauto with len.
+      * split; simpl; eauto.
       * pe_rewrite. set_simpl.
         rewrite List.map_app. rewrite list_union_app.
         eapply disj_union_left.
         -- symmetry.
            eapply funConstr_disj_Dt; eauto.
         -- symmetry. eapply disj_incl; eauto.
-      * revert LEN. clear; eauto with len.
-      * rewrite List.map_app.
-        eapply PIR2_app; eauto.
-        eapply PIR2_get; intros; inv_get. reflexivity.
-        clear.
-        eauto with len.
-      * intros ? ? GET. eapply get_app_cases in GET. destruct GET.
+      * intros ? ? GET2. eapply get_app_cases in GET2. destruct GET2.
         inv_get. edestruct H5; eauto.
         dcr. inv_get. eapply NODUP; eauto.
         Grab Existential Variables.
-        eapply subTerm_EQ_Fun2; eauto.
+        eauto.
+Qed.
+
+Definition cp_reachability_sound (sT:stmt)
+           ZL BL s (d:VDom (occurVars sT) _) r (ST:subTerm s sT) ZLIncl
+           (EQ:(fst (forward cp_trans cp_reach ZL ZLIncl s ST d r)) ≣ (d,r)) ra
+    (Ann: annotation s r) (RA:renamedApart s ra)
+    (DefZL: labelsDefined s (length ZL))
+    (DefBL: labelsDefined s (length BL))
+    (BL_le: poLe (snd (forward cp_trans cp_reach ZL ZLIncl s ST d r)) BL)
+    (Disj:disj (list_union (of_list ⊝ ZL)) (snd (getAnn ra)))
+  : reachability (cop2bool (domenv (proj1_sig d))) Sound BL s r.
+Proof.
+  eapply reachability_sound with (pr:=fun d => cop2bool (domenv (proj1_sig d)));
+    eauto using cp_trans_ext, cp_reach_ext.
+  - unfold cp_reach, cop2bool, Dom; intros;
+      repeat cases; simpl in *; unfold Dom in *; clear_trivial_eqs; eauto.
+    + exfalso. eapply H. rewrite COND; simpl. eauto.
+    + exfalso. eapply H. rewrite COND; simpl. eauto.
+    + exfalso. eapply H. rewrite COND; simpl. eauto.
+  - unfold cp_reach, cop2bool, Dom; intros;
+      repeat cases; simpl in *; unfold Dom in *; clear_trivial_eqs; eauto.
+    + exfalso. eapply H. rewrite COND; simpl. eauto.
+    + exfalso. eapply H. rewrite COND0; simpl. eauto.
+    + exfalso. eapply H. rewrite COND; simpl. eauto.
 Qed.
